Freigen.lean
@@ -2,4 +2,7 @@
 import Freigen.Free
 import Freigen.Ast
 import Freigen.Reflect
+import Freigen.Domain
+import Freigen.ITree
+import Freigen.DenoteITree
 import Freigen.Examples
